coq_inference/assert_tactics.v
@@ -4,18 +4,18 @@ Require Import L_def.
 Require Import exp.
 Require Import defs.
 Require Import operational_semantics.
-Require Import specw.
+Require Import assert.
 Require Import List.
 Require Export Coq.Lists.ListSet.
 
-Module SpecWTactics(L : LanguageDef).
+Module AssertTactics(L : LanguageDef).
 
   Import L.
-  Module L_SpecW := SpecW(L).
-  Export L_SpecW.
+  Module L_Assert := Assert(L).
+  Export L_Assert.
 
-  Open Scope specw_scope.
-  Declare Scope specw_tactics_scope.
+  Open Scope assert_scope.
+  Declare Scope assert_tactics_scope.
 
   Lemma aval_subst :
     forall x n v, ([x /s n](av_ v)) = (av_ v).
@@ -1041,4 +1041,4 @@ Module SpecWTactics(L : LanguageDef).
 
   Qed.
 
-End SpecWTactics.
+End AssertTactics.
