coq_inference/common.v
@@ -1,7 +1,7 @@
 Require Export Arith.
 Require Import List.
 
-Require Import chainmail.CpdtTactics.
+Require Import necessity.CpdtTactics.
 
 Class Eq (A : Type) :=
   {eqb : A -> A -> bool;
