coq_inference/hoare.v
@@ -5,9 +5,9 @@ Require Import L_def.
 Require Import exp.
 Require Import exp_properties.
 Require Import operational_semantics.
-Require Import specw.
+Require Import assert.
 Require Import classical.
-Require Import specw_inference.
+Require Import assert_proofsystem.
 Require Import List.
 Require Import String.
 Open Scope string_scope.
@@ -17,11 +17,11 @@ Require Import Coq.Logic.FunctionalExtensionality.
 Module Hoare(L : LanguageDef).
 
   Import L.
-  Module L_SpecWInf := SpecWInference(L).
-  Export L_SpecWInf.
+  Module L_AssertProofSystem := AssertProofSystem(L).
+  Export L_AssertProofSystem.
 
   Open Scope reduce_scope.
-  Open Scope specw_scope.
+  Open Scope assert_scope.
 
   Declare Scope hoare_scope.
 
@@ -56,6 +56,88 @@ Module Hoare(L : LanguageDef).
 
   Notation "M '⊢' '{pre:' P '}' m '{post:' Q '}'" := (hoare_triple M P m Q) (at level 40).
 
+  Inductive wf_value : config -> value -> Prop :=
+  | wf_true : forall σ, wf_value σ v_true
+  | wf_false : forall σ, wf_value σ v_false
+  | wf_null : forall σ, wf_value σ v_null
+  | wf_addr : forall χ ψ a, a ∈ χ ->
+                       wf_value (χ, ψ) (v_ a)
+  | wf_int : forall σ z, wf_value σ (v_int z).
+
+  Inductive wf_exp : config -> exp -> Prop :=
+  | wf_val : forall σ v, wf_value σ v ->
+                    wf_exp σ (e_val v)
+  | wf_var : forall σ x, wf_exp σ (e_var x)
+  | wf_hole : forall σ n, wf_exp σ (e_hole n)
+  | wf_eq : forall σ e1 e2, wf_exp σ e1 ->
+                       wf_exp σ e2 ->
+                       wf_exp σ (e_eq e1 e2)
+  | wf_lt : forall σ e1 e2, wf_exp σ e1 ->
+                       wf_exp σ e2 ->
+                       wf_exp σ (e_eq e1 e2)
+  | wf_plus : forall σ e1 e2, wf_exp σ e1 ->
+                         wf_exp σ e2 ->
+                         wf_exp σ (e_plus e1 e2)
+  | wf_minus : forall σ e1 e2, wf_exp σ e1 ->
+                          wf_exp σ e2 ->
+                          wf_exp σ (e_minus e1 e2)
+  | wf_mult : forall σ e1 e2, wf_exp σ e1 ->
+                         wf_exp σ e2 ->
+                         wf_exp σ (e_mult e1 e2)
+  | wf_div : forall σ e1 e2, wf_exp σ e1 ->
+                        wf_exp σ e2 ->
+                        wf_exp σ (e_div e1 e2)
+  | wf_if : forall σ e1 e2 e3, wf_exp σ e1 ->
+                          wf_exp σ e2 ->
+                          wf_exp σ e3 ->
+                          wf_exp σ (e_if e1 e2 e3)
+  | wf_acc_f : forall σ e f, wf_exp σ e ->
+                        wf_exp σ (e_acc_f e f)
+  | wf_acc_g : forall σ e1 g e2, wf_exp σ e1 ->
+                            wf_exp σ e2 ->
+                            wf_exp σ (e_acc_g e1 g e2).
+
+  Inductive wf_aval : config -> a_val -> Prop :=
+  | wf_ahole : forall σ n, wf_aval σ (a♢ n)
+  | wf_abnd : forall χ ψ a, a ∈ χ ->
+                       wf_aval (χ, ψ) (a_ a).
+
+  Definition wf_args (σ : config)(m : partial_map name a_val) : Prop :=
+    forall x a, ⟦ x ↦ a ⟧_∈ m ->
+           wf_aval σ a.
+
+  Inductive wf_asrt : config -> asrt -> Prop :=
+  | wf_expr : forall σ e,  wf_exp σ e ->
+                      wf_asrt σ (a_exp e)
+  | wf_class : forall σ e C, wf_exp σ e ->
+                        wf_asrt σ (a_class e C)
+  | wf_arr : forall σ A1 A2, wf_asrt σ A2 ->
+                        wf_asrt σ A1 ->
+                        wf_asrt σ (A1 ⟶ A2)
+  | wf_and : forall σ A1 A2, wf_asrt σ A2 ->
+                        wf_asrt σ A1 ->
+                        wf_asrt σ (A1 ∧ A2)
+  | wf_or : forall σ A1 A2, wf_asrt σ A2 ->
+                        wf_asrt σ A1 ->
+                        wf_asrt σ (A1 ∨ A2)
+  | wf_neg : forall σ A, wf_asrt σ A ->
+                    wf_asrt σ (¬ A)
+  | wf_all : forall σ A, wf_asrt σ A ->
+                    wf_asrt σ (∀x.[A])
+  | wf_ex : forall σ A, wf_asrt σ A ->
+                   wf_asrt σ (∃x.[A])
+  | wf_acc : forall σ a1 a2, wf_aval σ a1 ->
+                        wf_aval σ a2 ->
+                        wf_asrt σ (a1 access a2)
+  | wf_call : forall σ a1 a2 m args, wf_aval σ a1 ->
+                                wf_aval σ a2 ->
+                                wf_args σ args ->
+                                wf_asrt σ (a1 calls a2 ◌ m ⟨ args ⟩)
+  | wf_intrn : forall σ a, wf_aval σ a ->
+                      wf_asrt σ (a internal)
+  | wf_extrn : forall σ a, wf_aval σ a ->
+                      wf_asrt σ (a external).
+
   Inductive ht_semantics : mdl -> asrt -> meth_call -> asrt -> Prop :=
   | ht_r : forall M α m β P Q, (forall M' x σ σ', is_call σ x (m_call α m β) ->
                                         M ◎ σ ⊨ P ->
@@ -83,6 +165,6 @@ Module Hoare(L : LanguageDef).
     forall M x C m, M ⊢ {pre: a_class (e_ x) C} m {post: a_class (e_ x) C}.
 
   Close Scope hoare_scope.
-  Close Scope specw_scope.
+  Close Scope assert_scope.
   Close Scope reduce_scope.
 End Hoare.
